cfrontend/SimplLocalsproof.v
@@ -2907,6 +2907,7 @@ Proof.
       constructor; eauto.
 Qed.
 
+
 End PRESERVATION.
 
 Theorem transf_program_correct' prog tprog:
